nit

ulib/experimental/FStar.Reflection.Typing.fsti
@@ -1766,8 +1766,7 @@ val if_complete_match (g:env) (t:term)
 
 // Derived rule for if
 
-
-let mkif
+val mkif
     (g:fstar_env)
     (scrutinee:term)
     (then_:term)
@@ -1782,20 +1781,3 @@ let mkif
     (te : typing (extend_env g hyp (eq2 (pack_universe Uv_Zero) bool_ty scrutinee false_bool)) else_ (eff, ty))
     (tr : typing g ty (ty_eff, tm_type u_ty))
 : typing g (mk_if scrutinee then_ else_) (eff, ty)
-= let brt = (Pat_Constant C_True, then_) in
-  let bre = (Pat_Constant C_False, else_) in
-  bindings_ok_pat_constant g C_True;
-  bindings_ok_pat_constant g C_False;
-  let brty () : branches_typing g u_zero bool_ty scrutinee (eff,ty) [brt; bre] [[]; []] =
-    BT_S (Pat_Constant C_True, then_) []
-         (BO (Pat_Constant C_True) [] hyp then_ () tt)
-         _ _ (
-      BT_S (Pat_Constant C_False, else_) []
-           (BO (Pat_Constant C_False) [] hyp else_ () te)
-           _ _
-        BT_Nil)
-  in
-  T_Match g u_zero bool_ty scrutinee T.E_Total (T_FVar g bool_fv) eff ts [brt; bre] (eff, ty)
-    [[]; []]
-    (MC_Tok g scrutinee bool_ty _ _ (Squash.return_squash (if_complete_match g scrutinee)))
-    (brty ())
